ConcreteEvidence.v
@@ -1,0 +1,123 @@
+Require Import Term.
+
+Notation BS := nat (only parsing).
+
+(** * Concrete Evidence *)
+Inductive EvidenceC: Set :=
+| mtc: EvidenceC
+(*| sp: EvidenceC -> EvidenceC -> EvidenceC*)
+| kkc: ASP_ID -> (list Arg) -> (*Plc ->*) Plc -> BS -> EvidenceC -> EvidenceC
+| uuc: ASP_ID -> (list Arg) -> (*Plc ->*) BS -> EvidenceC -> EvidenceC
+| ggc: (*Plc ->*) EvidenceC -> BS -> EvidenceC
+| hhc: (*Plc ->*) BS -> EvidenceC -> EvidenceC
+| nnc: (*Plc ->*) N_ID -> BS -> EvidenceC -> EvidenceC
+| ssc: EvidenceC -> EvidenceC -> EvidenceC
+| ppc: EvidenceC -> EvidenceC -> EvidenceC.
+
+(** * Place-holder axioms for IO operations *)
+Definition invokeKIM (i:ASP_ID) (q:Plc) (args:list Arg) : BS.
+Admitted.
+Definition invokeUSM (i:ASP_ID) (args:list Arg) : BS.
+Admitted.
+Definition signEv (e:EvidenceC) : BS.
+Admitted.
+Definition hashEv (e:EvidenceC) : BS.
+Admitted.
+Definition toRemote (t:Term) (pTo:Plc) (e:EvidenceC) : EvidenceC.
+Admitted.
+Definition parallel_eval_thread (t:Term) (e:EvidenceC) : EvidenceC.
+Admitted.
+
+Fixpoint et_fun (p:Plc) (ec:EvidenceC) : Evidence :=
+  match ec with
+  | mtc => mt
+  | kkc i A q _ ec' => kk i A p q (et_fun p ec')
+  | uuc i A _ ec' => uu i A p (et_fun p ec')
+  | ggc ec' _ => gg p (et_fun p ec')
+  | hhc _ ec' => hh p (et_fun p ec')
+  | nnc n _ ec' => nn p n (et_fun p ec')
+  | ssc ec1 ec2 => ss (et_fun p ec1) (et_fun p ec2)
+  | ppc ec1 ec2 => pp (et_fun p ec1) (et_fun p ec2)
+  end.
+    
+(** * Types *)
+Inductive ET: Plc -> EvidenceC -> Evidence -> Prop :=
+| mtt: forall p, ET p mtc mt
+| kkt: forall id A p q bs e et,
+    ET p e et -> 
+    ET p (kkc id A q bs e) (kk id A p q et)
+| uut: forall id A p bs e et,
+    ET p e et -> 
+    ET p (uuc id A bs e) (uu id A p et)
+| ggt: forall p bs e et,
+    ET p e et ->
+    ET p (ggc e bs) (gg p et)
+| hht: forall p bs e et,
+    ET p e et ->
+    ET p (hhc bs e) (hh p et)
+| nnt: forall p bs e et i,
+    ET p e et ->
+    ET p (nnc i bs e) (nn p i et)
+| sst: forall p e1 e2 e1t e2t,
+    ET p e1 e1t ->
+    ET p e2 e2t ->
+    ET p (ssc e1 e2) (ss e1t e2t)
+| ppt: forall p e1 e2 e1t e2t,
+    ET p e1 e1t ->
+    ET p e2 e2t ->
+    ET p (ppc e1 e2) (pp e1t e2t).
+Hint Constructors ET.
+
+Theorem et_et_fun : forall p ec,
+    ET p ec (et_fun p ec).
+Proof.
+  intros.
+  generalize dependent p.
+  induction ec; intros; try (simpl; eauto).
+Defined.
+
+(** * Eval function definition *)
+Definition splitEv (sp:SP) (e:EvidenceC) : EvidenceC :=
+  match sp with
+  | ALL => e
+  | NONE => mtc
+  end.
+
+Definition eval_asp (a:ASP) (e:EvidenceC) : EvidenceC :=
+  match a with
+  | CPY => e
+  | KIM i q args =>
+    let bs := invokeKIM i q args in
+    (kkc i args q bs e)
+  | USM i args =>
+    let bs := invokeUSM i args in
+    (uuc i args bs e)
+  | SIG =>
+    let bs := signEv e in
+    (ggc e bs)
+  | HSH =>
+    let bs := hashEv e in
+    (hhc bs e)
+  end.
+
+Fixpoint eval (t:Term) (e:EvidenceC) : EvidenceC :=
+  match t with
+  | asp a => eval_asp a e
+  | att q t1 => toRemote t1 q e
+  | lseq t1 t2 =>
+    let e1 := eval t1 e in
+    eval t2 e1
+         
+  | bseq (sp1,sp2) t1 t2 =>
+    let e1 := splitEv sp1 e in
+    let e2 := splitEv sp2 e in
+    let e1' := eval t1 e1 in
+    let e2' := eval t2 e2 in
+    (ssc e1' e2') 
+  | bpar (sp1,sp2) t1 t2 =>
+    let e1 := splitEv sp1 e in
+    let e2 := splitEv sp2 e in
+    let e1' := parallel_eval_thread t1 e1 in
+    let e2' := parallel_eval_thread t2 e2 in
+    (ppc e1' e2')
+  end.
