VmSemantics.v
@@ -1,4 +1,4 @@
-Require Import More_lists Preamble Term LTS.
+Require Import More_lists Preamble Term ConcreteEvidence LTS.
 Require Import Instr MyStack MonadVM MonadVMFacts.
 
 Require Import List.
